passage examples en V8
git-svn-id: https://www.lri.fr/svn/demons/why2/trunk@586 ecafba89-7d34-45a1-8a0b-92829e960b72

examples/binary-search/bsearch_why.v
@@ -1,10 +1,10 @@
-
-Require Why.
-Require ZArith.
-Require Zcomplements.
-Require Omega. 
-
-Tactic Definition Omega' := Abstract Omega.
+(* Load Programs. *)
+Require Import Why.
+Require Import ZArith.
+Require Import Zcomplements.
+Require Import Omega.
+ 
+Ltac Omega' := abstract omega.
 
 (* Parameters and axioms *)
 
@@ -12,356 +12,369 @@ Tactic Definition Omega' := Abstract Omega.
 
 (* Specification *)
 
-Inductive In [t:(array Z); l,u:Z] : Prop :=
-  In_cons : (i:Z) `l <= i <= u` -> #t[i]=v -> (In t l u).
+Inductive In (t:array Z) (l u:Z) : Prop :=
+    In_cons : forall i:Z, (l <= i <= u)%Z -> access t i = v -> In t l u.
 
-Definition mean := [x,y:Z](Zdiv2 `x+y`).
+Definition mean (x y:Z) := Zdiv2 (x + y).
 
 (* Lemmas *)
 
-Lemma le_mean : (x,y:Z)
-  `0 <= x <= y` -> `x <= (mean x y)`.
+Lemma le_mean : forall x y:Z, (0 <= x <= y)%Z -> (x <= mean x y)%Z.
 Proof.
-Intros.
-Apply Zle_Zmult_right2 with z:=`2`.
-Omega.
-Rewrite Zmult_sym.
-Rewrite (Zmult_sym (mean x y) `2`).
-Unfold mean.
-Elim (Zeven_odd_dec `x+y`); Intro.
-Rewrite <- Zeven_div2 with `x+y`.
-Omega.
-Assumption.
-Elim (Z_eq_dec x y); Intro.
-Absurd x=y; Try Assumption.
-Rewrite a in b.
-Absurd (Zodd `y+y`); Try Assumption.
-Absurd `y+y = 2*(Zdiv2 (y+y))+1`.
-Omega.
-Apply Zodd_div2.
-Omega.
-Assumption.
-Cut `x+y = 2*(Zdiv2 (x+y))+1`.
-Omega.
-Apply Zodd_div2.
-Omega.
-Assumption.
-Save.
+intros.
+apply Zle_Zmult_right2 with (z := 2%Z).
+omega.
+rewrite Zmult_comm.
+rewrite (Zmult_comm (mean x y) 2).
+unfold mean.
+elim (Zeven_odd_dec (x + y)); intro.
+rewrite <- Zeven_div2 with (x + y)%Z.
+omega.
+assumption.
+elim (Z_eq_dec x y); intro.
+absurd (x = y); try assumption.
+rewrite a in b.
+absurd (Zodd (y + y)); try assumption.
+absurd ((y + y)%Z = (2 * Zdiv2 (y + y) + 1)%Z).
+omega.
+apply Zodd_div2.
+omega.
+assumption.
+cut ((x + y)%Z = (2 * Zdiv2 (x + y) + 1)%Z).
+omega.
+apply Zodd_div2.
+omega.
+assumption.
+Qed.
 
-Lemma ge_mean : (x,y:Z)
-  `0 <= x <= y` -> `(mean x y) <= y`.
+Lemma ge_mean : forall x y:Z, (0 <= x <= y)%Z -> (mean x y <= y)%Z.
 Proof.
-Intros.
-Apply Zle_Zmult_right2 with z:=`2`.
-Omega.
-Rewrite Zmult_sym.
-Rewrite (Zmult_sym y `2`).
-Unfold mean.
-Elim (Zeven_odd_dec `x+y`); Intro.
-Rewrite <- Zeven_div2 with `x+y`.
-Omega.
-Assumption.
-Cut `x+y = 2*(Zdiv2 (x+y))+1`.
-Omega.
-Apply Zodd_div2.
-Omega.
-Assumption.
-Save.
+intros.
+apply Zle_Zmult_right2 with (z := 2%Z).
+omega.
+rewrite Zmult_comm.
+rewrite (Zmult_comm y 2).
+unfold mean.
+elim (Zeven_odd_dec (x + y)); intro.
+rewrite <- Zeven_div2 with (x + y)%Z.
+omega.
+assumption.
+cut ((x + y)%Z = (2 * Zdiv2 (x + y) + 1)%Z).
+omega.
+apply Zodd_div2.
+omega.
+assumption.
+Qed.
 
-Lemma In_right_side : (t:(array Z))
-  (sorted_array t `1` `(array_length t)-1`) ->
-  (l,u:Z)
-  `1 <= l` -> `u <= (array_length t)-1` -> `l <= u` -> `l <= (mean l u) <= u` ->
-  ((In t `1` `(array_length t)-1`) -> (In t l u)) ->
-  `(access t (mean l u)) < v` ->
-  ((In t `1` `(array_length t)-1`) -> (In t `(mean l u)+1` u)).
-Proof.     
-Intros t Hsorted l u Hl Hu Hlu Hm Inv Hv H.
-Generalize (Inv H). Intro.
-Decompose [In] H0.
-Apply In_cons with i.
-Elim (Z_gt_le_dec `(mean l u)+1` i); Intro.
-Absurd (access t i)=v.
-Apply Zlt_not_eq.
-Apply Zle_lt_trans with (access t (mean l u)).
-Apply sorted_elements with n:=`1` m:=`(array_length t)-1`.
-Assumption.
+Lemma In_right_side :
+ forall t:array Z,
+   sorted_array t 1 (array_length t - 1) ->
+   forall l u:Z,
+     (1 <= l)%Z ->
+     (u <= array_length t - 1)%Z ->
+     (l <= u)%Z ->
+     (l <= mean l u <= u)%Z ->
+     (In t 1 (array_length t - 1) -> In t l u) ->
+     (access t (mean l u) < v)%Z ->
+     In t 1 (array_length t - 1) -> In t (mean l u + 1) u.
+     Proof.
+     intros t Hsorted l u Hl Hu Hlu Hm Inv Hv H.
+generalize (Inv H).
+ intro.
+decompose [In] H0.
+apply In_cons with i.
+elim (Z_gt_le_dec (mean l u + 1) i); intro.
+absurd (access t i = v).
+apply Zlt_not_eq.
+apply Zle_lt_trans with (access t (mean l u)).
+apply sorted_elements with (n := 1%Z) (m := (array_length t - 1)%Z).
+assumption.
 Omega'.
 Omega'.
 Omega'.
 Omega'.
-Assumption.
-Assumption.
+assumption.
+assumption.
 Omega'.
-Assumption.
-Save.
+assumption.
+Qed.
 
-Lemma In_left_side : (t:(array Z))
-  (sorted_array t `1` `(array_length t)-1`) ->
-  (l,u:Z)
-  `1 <= l` -> `u <= (array_length t)-1` -> `l <= u` -> `l <= (mean l u) <= u` ->
-  ((In t `1` `(array_length t)-1`) -> (In t l u)) ->
-  `(access t (mean l u)) > v` ->
-  ((In t `1` `(array_length t)-1`) -> (In t l `(mean l u)-1`)).
-Proof.     
-Intros t Hsorted l u Hl Hu Hlu Hm Inv Hv H.
-Generalize (Inv H). Intro.
-Decompose [In] H0.
-Apply In_cons with i.
-Elim (Z_gt_le_dec i `(mean l u)-1`); Intro.
-Absurd (access t i)=v.
-Apply sym_not_eq.
-Apply Zlt_not_eq.
-Apply Zlt_le_trans with (access t (mean l u)).
+Lemma In_left_side :
+ forall t:array Z,
+   sorted_array t 1 (array_length t - 1) ->
+   forall l u:Z,
+     (1 <= l)%Z ->
+     (u <= array_length t - 1)%Z ->
+     (l <= u)%Z ->
+     (l <= mean l u <= u)%Z ->
+     (In t 1 (array_length t - 1) -> In t l u) ->
+     (access t (mean l u) > v)%Z ->
+     In t 1 (array_length t - 1) -> In t l (mean l u - 1).
+     Proof.
+     intros t Hsorted l u Hl Hu Hlu Hm Inv Hv H.
+generalize (Inv H).
+ intro.
+decompose [In] H0.
+apply In_cons with i.
+elim (Z_gt_le_dec i (mean l u - 1)); intro.
+absurd (access t i = v).
+apply sym_not_eq.
+apply Zlt_not_eq.
+apply Zlt_le_trans with (access t (mean l u)).
 Omega'.
-Apply sorted_elements with n:=`1` m:=`(array_length t)-1`.
-Assumption.
+apply sorted_elements with (n := 1%Z) (m := (array_length t - 1)%Z).
+assumption.
 Omega'.
 Omega'.
 Omega'.
 Omega'.
-Assumption.
+assumption.
 Omega'.
-Assumption.
-Save.
+assumption.
+Qed.
 
 (* Obligations *)
 
 (* Why obligation from file "bsearch.mlw", characters 557-574 *)
 Lemma binary_search_po_1 : 
-  (t: (array Z))
-  (Pre15: `(array_length t) >= 1` /\
-          (sorted_array t `1` `(array_length t) - 1`))
-  (l0: Z)
-  (Post1: l0 = `1`)
-  (u0: Z)
-  (Post2: u0 = `(array_length t) - 1`)
-  (p0: Z)
-  (Post3: p0 = `0`)
-  (Variant1: Z)
-  (l1: Z)
-  (p1: Z)
-  (u1: Z)
-  (Pre14: Variant1 = `2 + u1 - l1`)
-  (Pre13: `1 <= l1` /\ `u1 <= (array_length t) - 1` /\ (`0 <= p1` /\
-          `p1 <= (array_length t) - 1`) /\
-          ((`p1 = 0` -> ((In t `1` `(array_length t) - 1`) -> (In t l1 u1)))) /\
-          ((`p1 > 0` -> `(access t p1) = v`)))
-  (Test6: `l1 <= u1`)
-  (m1: Z)
-  (Post4: m1 = (mean l1 u1))
-  `l1 <= m1` /\ `m1 <= u1`.
-Proof. 
-Intros.
-Split. Rewrite Post4; Apply le_mean; Omega'.
-Rewrite Post4; Apply ge_mean; Omega'.
-Save.
+  forall (t: (array Z)),
+  forall (Pre15: (array_length t) >= 1 /\
+                 (sorted_array t 1 ((array_length t) - 1))),
+  forall (l0: Z),
+  forall (Post1: l0 = 1),
+  forall (u0: Z),
+  forall (Post2: u0 = ((array_length t) - 1)),
+  forall (p0: Z),
+  forall (Post3: p0 = 0),
+  forall (Variant1: Z),
+  forall (l1: Z),
+  forall (p1: Z),
+  forall (u1: Z),
+  forall (Pre14: Variant1 = (2 + u1 - l1)),
+  forall (Pre13: 1 <= l1 /\ u1 <= ((array_length t) - 1) /\ (0 <= p1 /\ p1 <=
+                 ((array_length t) - 1)) /\
+                 ((p1 = 0 ->
+                   ((In t 1 ((array_length t) - 1)) -> (In t l1 u1)))) /\
+                 ((p1 > 0 -> (access t p1) = v))),
+  forall (Test6: l1 <= u1),
+  forall (m1: Z),
+  forall (Post4: m1 = (mean l1 u1)),
+  l1 <= m1 /\ m1 <= u1.
+ Proof.
+ intros.
+split.
+ rewrite Post4; apply le_mean; Omega'.
+rewrite Post4; apply ge_mean; Omega'.
+Qed.
 
 (* Why obligation from file "bsearch.mlw", characters 587-592 *)
 Lemma binary_search_po_2 : 
-  (t: (array Z))
-  (Pre15: `(array_length t) >= 1` /\
-          (sorted_array t `1` `(array_length t) - 1`))
-  (l0: Z)
-  (Post1: l0 = `1`)
-  (u0: Z)
-  (Post2: u0 = `(array_length t) - 1`)
-  (p0: Z)
-  (Post3: p0 = `0`)
-  (Variant1: Z)
-  (l1: Z)
-  (p1: Z)
-  (u1: Z)
-  (Pre14: Variant1 = `2 + u1 - l1`)
-  (Pre13: `1 <= l1` /\ `u1 <= (array_length t) - 1` /\ (`0 <= p1` /\
-          `p1 <= (array_length t) - 1`) /\
-          ((`p1 = 0` -> ((In t `1` `(array_length t) - 1`) -> (In t l1 u1)))) /\
-          ((`p1 > 0` -> `(access t p1) = v`)))
-  (Test6: `l1 <= u1`)
-  (m1: Z)
-  (Post4: m1 = (mean l1 u1))
-  (Pre12: `l1 <= m1` /\ `m1 <= u1`)
-  `0 <= m1` /\ `m1 < (array_length t)`.
+  forall (t: (array Z)),
+  forall (Pre15: (array_length t) >= 1 /\
+                 (sorted_array t 1 ((array_length t) - 1))),
+  forall (l0: Z),
+  forall (Post1: l0 = 1),
+  forall (u0: Z),
+  forall (Post2: u0 = ((array_length t) - 1)),
+  forall (p0: Z),
+  forall (Post3: p0 = 0),
+  forall (Variant1: Z),
+  forall (l1: Z),
+  forall (p1: Z),
+  forall (u1: Z),
+  forall (Pre14: Variant1 = (2 + u1 - l1)),
+  forall (Pre13: 1 <= l1 /\ u1 <= ((array_length t) - 1) /\ (0 <= p1 /\ p1 <=
+                 ((array_length t) - 1)) /\
+                 ((p1 = 0 ->
+                   ((In t 1 ((array_length t) - 1)) -> (In t l1 u1)))) /\
+                 ((p1 > 0 -> (access t p1) = v))),
+  forall (Test6: l1 <= u1),
+  forall (m1: Z),
+  forall (Post4: m1 = (mean l1 u1)),
+  forall (Pre12: l1 <= m1 /\ m1 <= u1),
+  0 <= m1 /\ m1 < (array_length t).
 Proof.
-Intros.
+intros.
 Omega'.
-Save.
+Qed.
 
 (* Why obligation from file "bsearch.mlw", characters 610-621 *)
 Lemma binary_search_po_3 : 
-  (t: (array Z))
-  (Pre15: `(array_length t) >= 1` /\
-          (sorted_array t `1` `(array_length t) - 1`))
-  (l0: Z)
-  (Post1: l0 = `1`)
-  (u0: Z)
-  (Post2: u0 = `(array_length t) - 1`)
-  (p0: Z)
-  (Post3: p0 = `0`)
-  (Variant1: Z)
-  (l1: Z)
-  (p1: Z)
-  (u1: Z)
-  (Pre14: Variant1 = `2 + u1 - l1`)
-  (Pre13: `1 <= l1` /\ `u1 <= (array_length t) - 1` /\ (`0 <= p1` /\
-          `p1 <= (array_length t) - 1`) /\
-          ((`p1 = 0` -> ((In t `1` `(array_length t) - 1`) -> (In t l1 u1)))) /\
-          ((`p1 > 0` -> `(access t p1) = v`)))
-  (Test6: `l1 <= u1`)
-  (m1: Z)
-  (Post4: m1 = (mean l1 u1))
-  (Pre12: `l1 <= m1` /\ `m1 <= u1`)
-  (Pre11: `0 <= m1` /\ `m1 < (array_length t)`)
-  (Test5: `(access t m1) < v`)
-  (l2: Z)
-  (Post5: l2 = `m1 + 1`)
-  (`1 <= l2` /\ `u1 <= (array_length t) - 1` /\ (`0 <= p1` /\
-  `p1 <= (array_length t) - 1`) /\
-  ((`p1 = 0` -> ((In t `1` `(array_length t) - 1`) -> (In t l2 u1)))) /\
-  ((`p1 > 0` -> `(access t p1) = v`))) /\
-  (Zwf `0` `2 + u1 - l2` `2 + u1 - l1`).
+  forall (t: (array Z)),
+  forall (Pre15: (array_length t) >= 1 /\
+                 (sorted_array t 1 ((array_length t) - 1))),
+  forall (l0: Z),
+  forall (Post1: l0 = 1),
+  forall (u0: Z),
+  forall (Post2: u0 = ((array_length t) - 1)),
+  forall (p0: Z),
+  forall (Post3: p0 = 0),
+  forall (Variant1: Z),
+  forall (l1: Z),
+  forall (p1: Z),
+  forall (u1: Z),
+  forall (Pre14: Variant1 = (2 + u1 - l1)),
+  forall (Pre13: 1 <= l1 /\ u1 <= ((array_length t) - 1) /\ (0 <= p1 /\ p1 <=
+                 ((array_length t) - 1)) /\
+                 ((p1 = 0 ->
+                   ((In t 1 ((array_length t) - 1)) -> (In t l1 u1)))) /\
+                 ((p1 > 0 -> (access t p1) = v))),
+  forall (Test6: l1 <= u1),
+  forall (m1: Z),
+  forall (Post4: m1 = (mean l1 u1)),
+  forall (Pre12: l1 <= m1 /\ m1 <= u1),
+  forall (Pre11: 0 <= m1 /\ m1 < (array_length t)),
+  forall (Test5: (access t m1) < v),
+  forall (l2: Z),
+  forall (Post5: l2 = (m1 + 1)),
+  (1 <= l2 /\ u1 <= ((array_length t) - 1) /\ (0 <= p1 /\ p1 <=
+  ((array_length t) - 1)) /\
+  ((p1 = 0 -> ((In t 1 ((array_length t) - 1)) -> (In t l2 u1)))) /\
+  ((p1 > 0 -> (access t p1) = v))) /\ (Zwf 0 (2 + u1 - l2) (2 + u1 - l1)).
 Proof.
-Intros.
-Repeat Split; Try Omega'.
-Subst l2 m1.
-Intros; Apply In_right_side; Assumption Orelse Intuition.
-Save.
+intros.
+repeat split; try Omega'.
+subst l2 m1.
+intros; apply In_right_side; assumption || intuition.
+Qed.
 
 (* Why obligation from file "bsearch.mlw", characters 659-670 *)
 Lemma binary_search_po_4 : 
-  (t: (array Z))
-  (Pre15: `(array_length t) >= 1` /\
-          (sorted_array t `1` `(array_length t) - 1`))
-  (l0: Z)
-  (Post1: l0 = `1`)
-  (u0: Z)
-  (Post2: u0 = `(array_length t) - 1`)
-  (p0: Z)
-  (Post3: p0 = `0`)
-  (Variant1: Z)
-  (l1: Z)
-  (p1: Z)
-  (u1: Z)
-  (Pre14: Variant1 = `2 + u1 - l1`)
-  (Pre13: `1 <= l1` /\ `u1 <= (array_length t) - 1` /\ (`0 <= p1` /\
-          `p1 <= (array_length t) - 1`) /\
-          ((`p1 = 0` -> ((In t `1` `(array_length t) - 1`) -> (In t l1 u1)))) /\
-          ((`p1 > 0` -> `(access t p1) = v`)))
-  (Test6: `l1 <= u1`)
-  (m1: Z)
-  (Post4: m1 = (mean l1 u1))
-  (Pre12: `l1 <= m1` /\ `m1 <= u1`)
-  (Pre11: `0 <= m1` /\ `m1 < (array_length t)`)
-  (Test4: `(access t m1) >= v`)
-  (Pre10: `0 <= m1` /\ `m1 < (array_length t)`)
-  (Test3: `(access t m1) > v`)
-  (u2: Z)
-  (Post6: u2 = `m1 - 1`)
-  (`1 <= l1` /\ `u2 <= (array_length t) - 1` /\ (`0 <= p1` /\
-  `p1 <= (array_length t) - 1`) /\
-  ((`p1 = 0` -> ((In t `1` `(array_length t) - 1`) -> (In t l1 u2)))) /\
-  ((`p1 > 0` -> `(access t p1) = v`))) /\
-  (Zwf `0` `2 + u2 - l1` `2 + u1 - l1`).
+  forall (t: (array Z)),
+  forall (Pre15: (array_length t) >= 1 /\
+                 (sorted_array t 1 ((array_length t) - 1))),
+  forall (l0: Z),
+  forall (Post1: l0 = 1),
+  forall (u0: Z),
+  forall (Post2: u0 = ((array_length t) - 1)),
+  forall (p0: Z),
+  forall (Post3: p0 = 0),
+  forall (Variant1: Z),
+  forall (l1: Z),
+  forall (p1: Z),
+  forall (u1: Z),
+  forall (Pre14: Variant1 = (2 + u1 - l1)),
+  forall (Pre13: 1 <= l1 /\ u1 <= ((array_length t) - 1) /\ (0 <= p1 /\ p1 <=
+                 ((array_length t) - 1)) /\
+                 ((p1 = 0 ->
+                   ((In t 1 ((array_length t) - 1)) -> (In t l1 u1)))) /\
+                 ((p1 > 0 -> (access t p1) = v))),
+  forall (Test6: l1 <= u1),
+  forall (m1: Z),
+  forall (Post4: m1 = (mean l1 u1)),
+  forall (Pre12: l1 <= m1 /\ m1 <= u1),
+  forall (Pre11: 0 <= m1 /\ m1 < (array_length t)),
+  forall (Test4: (access t m1) >= v),
+  forall (Pre10: 0 <= m1 /\ m1 < (array_length t)),
+  forall (Test3: (access t m1) > v),
+  forall (u2: Z),
+  forall (Post6: u2 = (m1 - 1)),
+  (1 <= l1 /\ u2 <= ((array_length t) - 1) /\ (0 <= p1 /\ p1 <=
+  ((array_length t) - 1)) /\
+  ((p1 = 0 -> ((In t 1 ((array_length t) - 1)) -> (In t l1 u2)))) /\
+  ((p1 > 0 -> (access t p1) = v))) /\ (Zwf 0 (2 + u2 - l1) (2 + u1 - l1)).
 Proof.
-Intuition.
-Subst u2 m1.
-Intros; Apply In_left_side; Assumption Orelse Intuition.
-Save.
+intuition.
+subst u2 m1.
+intros; apply In_left_side; assumption || intuition.
+Qed.
 
 (* Why obligation from file "bsearch.mlw", characters 682-741 *)
 Lemma binary_search_po_5 : 
-  (t: (array Z))
-  (Pre15: `(array_length t) >= 1` /\
-          (sorted_array t `1` `(array_length t) - 1`))
-  (l0: Z)
-  (Post1: l0 = `1`)
-  (u0: Z)
-  (Post2: u0 = `(array_length t) - 1`)
-  (p0: Z)
-  (Post3: p0 = `0`)
-  (Variant1: Z)
-  (l1: Z)
-  (p1: Z)
-  (u1: Z)
-  (Pre14: Variant1 = `2 + u1 - l1`)
-  (Pre13: `1 <= l1` /\ `u1 <= (array_length t) - 1` /\ (`0 <= p1` /\
-          `p1 <= (array_length t) - 1`) /\
-          ((`p1 = 0` -> ((In t `1` `(array_length t) - 1`) -> (In t l1 u1)))) /\
-          ((`p1 > 0` -> `(access t p1) = v`)))
-  (Test6: `l1 <= u1`)
-  (m1: Z)
-  (Post4: m1 = (mean l1 u1))
-  (Pre12: `l1 <= m1` /\ `m1 <= u1`)
-  (Pre11: `0 <= m1` /\ `m1 < (array_length t)`)
-  (Test4: `(access t m1) >= v`)
-  (Pre10: `0 <= m1` /\ `m1 < (array_length t)`)
-  (Test2: `(access t m1) <= v`)
-  (p2: Z)
-  (Post7: p2 = m1)
-  (l2: Z)
-  (Post8: l2 = `u1 + 1`)
-  (`1 <= l2` /\ `u1 <= (array_length t) - 1` /\ (`0 <= p2` /\
-  `p2 <= (array_length t) - 1`) /\
-  ((`p2 = 0` -> ((In t `1` `(array_length t) - 1`) -> (In t l2 u1)))) /\
-  ((`p2 > 0` -> `(access t p2) = v`))) /\
-  (Zwf `0` `2 + u1 - l2` `2 + u1 - l1`).
+  forall (t: (array Z)),
+  forall (Pre15: (array_length t) >= 1 /\
+                 (sorted_array t 1 ((array_length t) - 1))),
+  forall (l0: Z),
+  forall (Post1: l0 = 1),
+  forall (u0: Z),
+  forall (Post2: u0 = ((array_length t) - 1)),
+  forall (p0: Z),
+  forall (Post3: p0 = 0),
+  forall (Variant1: Z),
+  forall (l1: Z),
+  forall (p1: Z),
+  forall (u1: Z),
+  forall (Pre14: Variant1 = (2 + u1 - l1)),
+  forall (Pre13: 1 <= l1 /\ u1 <= ((array_length t) - 1) /\ (0 <= p1 /\ p1 <=
+                 ((array_length t) - 1)) /\
+                 ((p1 = 0 ->
+                   ((In t 1 ((array_length t) - 1)) -> (In t l1 u1)))) /\
+                 ((p1 > 0 -> (access t p1) = v))),
+  forall (Test6: l1 <= u1),
+  forall (m1: Z),
+  forall (Post4: m1 = (mean l1 u1)),
+  forall (Pre12: l1 <= m1 /\ m1 <= u1),
+  forall (Pre11: 0 <= m1 /\ m1 < (array_length t)),
+  forall (Test4: (access t m1) >= v),
+  forall (Pre10: 0 <= m1 /\ m1 < (array_length t)),
+  forall (Test2: (access t m1) <= v),
+  forall (p2: Z),
+  forall (Post7: p2 = m1),
+  forall (l2: Z),
+  forall (Post8: l2 = (u1 + 1)),
+  (1 <= l2 /\ u1 <= ((array_length t) - 1) /\ (0 <= p2 /\ p2 <=
+  ((array_length t) - 1)) /\
+  ((p2 = 0 -> ((In t 1 ((array_length t) - 1)) -> (In t l2 u1)))) /\
+  ((p2 > 0 -> (access t p2) = v))) /\ (Zwf 0 (2 + u1 - l2) (2 + u1 - l1)).
 Proof.
-Intuition.
-Absurd `p2 = 0`; Omega'.
-Subst p2; Omega.
-Save.
+intuition.
+absurd (p2 = 0%Z); Omega'.
+subst p2; omega.
+Qed.
 
 (* Why obligation from file "bsearch.mlw", characters 331-492 *)
 Lemma binary_search_po_6 : 
-  (t: (array Z))
-  (Pre15: `(array_length t) >= 1` /\
-          (sorted_array t `1` `(array_length t) - 1`))
-  (l0: Z)
-  (Post1: l0 = `1`)
-  (u0: Z)
-  (Post2: u0 = `(array_length t) - 1`)
-  (p0: Z)
-  (Post3: p0 = `0`)
-  `1 <= l0` /\ `u0 <= (array_length t) - 1` /\ (`0 <= p0` /\
-  `p0 <= (array_length t) - 1`) /\
-  ((`p0 = 0` -> ((In t `1` `(array_length t) - 1`) -> (In t l0 u0)))) /\
-  ((`p0 > 0` -> `(access t p0) = v`)).
+  forall (t: (array Z)),
+  forall (Pre15: (array_length t) >= 1 /\
+                 (sorted_array t 1 ((array_length t) - 1))),
+  forall (l0: Z),
+  forall (Post1: l0 = 1),
+  forall (u0: Z),
+  forall (Post2: u0 = ((array_length t) - 1)),
+  forall (p0: Z),
+  forall (Post3: p0 = 0),
+  1 <= l0 /\ u0 <= ((array_length t) - 1) /\ (0 <= p0 /\ p0 <=
+  ((array_length t) - 1)) /\
+  ((p0 = 0 -> ((In t 1 ((array_length t) - 1)) -> (In t l0 u0)))) /\
+  ((p0 > 0 -> (access t p0) = v)).
 Proof.
-Intuition.
-Subst l0 u0; Assumption.
-Save.
+intuition.
+subst l0 u0; assumption.
+Qed.
 
 (* Why obligation from file "bsearch.mlw", characters 169-860 *)
 Lemma binary_search_po_7 : 
-  (t: (array Z))
-  (Pre15: `(array_length t) >= 1` /\
-          (sorted_array t `1` `(array_length t) - 1`))
-  (l0: Z)
-  (Post1: l0 = `1`)
-  (u0: Z)
-  (Post2: u0 = `(array_length t) - 1`)
-  (p0: Z)
-  (Post3: p0 = `0`)
-  (l1: Z)
-  (p1: Z)
-  (u1: Z)
-  (Post9: (`1 <= l1` /\ `u1 <= (array_length t) - 1` /\ (`0 <= p1` /\
-          `p1 <= (array_length t) - 1`) /\
-          ((`p1 = 0` -> ((In t `1` `(array_length t) - 1`) -> (In t l1 u1)))) /\
-          ((`p1 > 0` -> `(access t p1) = v`))) /\ `l1 > u1`)
-  (`1 <= p1` /\ `p1 <= (array_length t) - 1`) /\ `(access t p1) = v` \/
-  `p1 = 0` /\ ~(In t `1` `(array_length t) - 1`).
+  forall (t: (array Z)),
+  forall (Pre15: (array_length t) >= 1 /\
+                 (sorted_array t 1 ((array_length t) - 1))),
+  forall (l0: Z),
+  forall (Post1: l0 = 1),
+  forall (u0: Z),
+  forall (Post2: u0 = ((array_length t) - 1)),
+  forall (p0: Z),
+  forall (Post3: p0 = 0),
+  forall (l1: Z),
+  forall (p1: Z),
+  forall (u1: Z),
+  forall (Post9: (1 <= l1 /\ u1 <= ((array_length t) - 1) /\ (0 <= p1 /\
+                 p1 <= ((array_length t) - 1)) /\
+                 ((p1 = 0 ->
+                   ((In t 1 ((array_length t) - 1)) -> (In t l1 u1)))) /\
+                 ((p1 > 0 -> (access t p1) = v))) /\ l1 > u1),
+  (1 <= p1 /\ p1 <= ((array_length t) - 1)) /\ (access t p1) = v \/ p1 = 0 /\
+  ~(In t 1 ((array_length t) - 1)).
 Proof.
-Intuition.
-Elim (Z_lt_ge_dec `0` p1); Intro.
-Left; Omega'.
-Right. 
-Cut `p1 = 0`; [ Intro | Omega' ].
-Split. Assumption.
-Intro. 
-Generalize (H4 H6 H9); Intro.
-Decompose [In] H10.
-Absurd `l1 <= i <= u1`; Omega'.
-Save.
+intuition.
+elim (Z_lt_ge_dec 0 p1); intro.
+left; Omega'.
+right.
+ cut (p1 = 0%Z); [ intro | Omega' ].
+split.
+ assumption.
+intro.
+ generalize (H4 H6 H9); intro.
+decompose [In] H10.
+absurd (l1 <= i <= u1)%Z; Omega'.
+Qed.
 
 
